wip

DY/Actions/Compromise.lean
@@ -10,9 +10,32 @@ import DY.Step
 
 namespace DY.Compromise
 
+section Execution
+
 public
 structure CompromiseEvent (StateT: Type) where
   state: StateT
+
+@[expose]
+public
+def ExecEntryT.internal (StateT: Type): Fin 1 → Type
+  | 0 => ProtocolEvent.ExecEntryT (CompromiseEvent StateT)
+
+public
+abbrev ExecEntryT (StateT: Type): Type :=
+  ExecTraceTypes.combine (ExecEntryT.internal StateT)
+
+public
+instance (StateT: Type): ExecTraceTypes.HasStep (ProtocolEvent.ExecEntryT (CompromiseEvent StateT)) (ExecEntryT StateT) :=
+  inferInstanceAs (ExecTraceTypes.HasStep (ExecEntryT.internal StateT 0) (ExecTraceTypes.combine (ExecEntryT.internal StateT)))
+
+public
+def baseAttackerKnowledge.internal [BytesFunctor] [ExecTraceTypes] (StateT: Type): (id: Fin 1) → SubBaseAttackerKnowledge (ExecEntryT.internal StateT id)
+  | 0 => ProtocolEvent.baseAttackerKnowledge (CompromiseEvent StateT)
+
+public
+def baseAttackerKnowledge [BytesFunctor] [ExecTraceTypes] (StateT: Type): SubBaseAttackerKnowledge (ExecEntryT StateT) :=
+  SubBaseAttackerKnowledge.combine (baseAttackerKnowledge.internal StateT)
 
 public
 def compromise
@@ -22,7 +45,7 @@ def compromise
   [ExecTraceTypes]
   [ExecTraceTypes.Has Network.ExecEntryT]
   [ExecTraceTypes.Has (PersistentGlobalState.ExecEntryT StateT)]
-  [ExecTraceTypes.Has (ProtocolEvent.ExecEntryT (CompromiseEvent StateT))]
+  [ExecTraceTypes.Has (ExecEntryT StateT)]
   (i: Nat)
   : Traceful Nat
 := do
@@ -33,7 +56,7 @@ def compromise
 public
 def GlobalStateCompromised
   {StateT: Type}
-  [ExecTraceTypes] [ExecTraceTypes.Has (ProtocolEvent.ExecEntryT (CompromiseEvent StateT))]
+  [ExecTraceTypes] [ExecTraceTypes.Has (ExecEntryT StateT)]
   (state: StateT)
   (tr: ExecTrace)
   : Prop
@@ -43,7 +66,7 @@ def GlobalStateCompromised
 public
 theorem GlobalStateCompromised_le
   {StateT: Type}
-  [ExecTraceTypes] [ExecTraceTypes.Has (ProtocolEvent.ExecEntryT (CompromiseEvent StateT))]
+  [ExecTraceTypes] [ExecTraceTypes.Has (ExecEntryT StateT)]
   (state: StateT)
   (tr1 tr2: ExecTrace)
   : tr1 ≤ tr2 →
@@ -55,10 +78,76 @@ theorem GlobalStateCompromised_le
 
 grind_pattern GlobalStateCompromised_le => tr1 ≤ tr2, GlobalStateCompromised state tr1
 
+end Execution
+
+section Proof
+
+@[expose]
+public
+def ProofEntryT.internal (StateT: Type): Fin 1 → Type
+  | 0 => ProtocolEvent.ProofEntryT (CompromiseEvent StateT)
+
+public
+abbrev ProofEntryT (StateT: Type): Type :=
+  TraceTypes.combine (ProofEntryT.internal StateT)
+
+public
+instance (StateT: Type): ∀ id, ErasableProofEntry (ExecEntryT.internal StateT id) (ProofEntryT.internal StateT id)
+  | 0 => by dsimp only [ExecEntryT.internal, ProofEntryT.internal]; infer_instance
+
+public
+instance (StateT: Type): ErasableProofEntry (ExecEntryT StateT) (ProofEntryT StateT) := by
+  dsimp only [ExecEntryT, ProofEntryT]
+  infer_instance
+
+public
+instance (StateT: Type): TraceTypes.HasStep (ProtocolEvent.ProofEntryT (CompromiseEvent StateT)) (ProofEntryT StateT) :=
+  inferInstanceAs (TraceTypes.HasStep (ProofEntryT.internal StateT 0) (TraceTypes.combine (ProofEntryT.internal StateT)))
+
+public
+instance
+  {StateT: Type}
+  [TraceTypes]
+  : ProtocolEvent.EventInv (CompromiseEvent StateT)
+where
+  invariant _ _ := True
+
+public
+instance [TraceTypes] (StateT: Type): ∀ id, ProofEntryInvariant (ProofEntryT.internal StateT id)
+  | 0 => by dsimp only [ProofEntryT.internal]; infer_instance
+
+public
+instance [TraceTypes] (StateT: Type): ProofEntryInvariant (ProofEntryT StateT) := by dsimp only [ProofEntryT]; infer_instance
+
+public
+instance [TraceTypes] (StateT: Type): TraceInvariant.HasStep (ProtocolEvent.ProofEntryT (CompromiseEvent StateT)) (ProofEntryT StateT) :=
+  inferInstanceAs (TraceInvariant.HasStep (ProofEntryT.internal StateT 0) (TraceTypes.combine (ProofEntryT.internal StateT)))
+
+public
+instance
+  [TraceInvariant] [BytesFunctor] [BytesInvariants]
+  (StateT: Type)
+  [TraceTypes.Has (ProofEntryT StateT)]
+  [TraceInvariant.Has (ProofEntryT StateT)]
+  : ∀ id, SubBaseAttackerKnowledgeTheorem (ProofEntryT.internal StateT id) (baseAttackerKnowledge.internal StateT id)
+  -- TODO: investigate why infer_instance doesn't work
+  | 0 => by dsimp only [ProofEntryT.internal, baseAttackerKnowledge.internal]; apply ProtocolEvent.baseAttackerKnowledgeTheorem
+
+public
+instance baseAttackerKnowledgeTheorem
+  [TraceInvariant] [BytesFunctor] [BytesInvariants]
+  (StateT: Type)
+  [TraceTypes.Has (ProofEntryT StateT)]
+  [TraceInvariant.Has (ProofEntryT StateT)]
+  : SubBaseAttackerKnowledgeTheorem (ProofEntryT StateT) (baseAttackerKnowledge StateT)
+:= by
+  dsimp only [ProofEntryT, baseAttackerKnowledge]
+  infer_instance
+
 public
 def label
   {StateT: Type}
-  [ExecTraceTypes] [ExecTraceTypes.Has (ProtocolEvent.ExecEntryT (CompromiseEvent StateT))]
+  [ExecTraceTypes] [ExecTraceTypes.Has (ExecEntryT StateT)]
   (state: StateT)
 :=
   ProtocolEvent.label ({ state }: CompromiseEvent StateT)
@@ -66,7 +155,7 @@ def label
 public
 theorem label_isCorrupt
   {StateT: Type}
-  [ExecTraceTypes] [ExecTraceTypes.Has (ProtocolEvent.ExecEntryT (CompromiseEvent StateT))]
+  [ExecTraceTypes] [ExecTraceTypes.Has (ExecEntryT StateT)]
   (state: StateT)
   (tr: ExecTrace)
   : (label state).isCorrupt tr = GlobalStateCompromised state tr
@@ -82,20 +171,12 @@ class CompromisableStateInv
   [BytesFunctor] [BytesInvariants]
   [Comparse.ParseableSerializeable StateT]
   [PersistentGlobalState.GlobalStateInv StateT]
-  [ExecTraceTypes.Has (ProtocolEvent.ExecEntryT (CompromiseEvent StateT))]
+  [ExecTraceTypes.Has (ExecEntryT StateT)]
 where
   invariant_implies_KnowableBy:
     ∀ (state: StateT) tr,
       PersistentGlobalState.GlobalStateInv.invariant state tr →
       Comparse.isWellFormed (Bytes.KnowableBy (label state)) state tr
-
-public
-instance
-  {StateT: Type}
-  [TraceTypes]
-  : ProtocolEvent.EventInv (CompromiseEvent StateT)
-where
-  invariant _ _ := True
 
 @[instance]
 public
@@ -105,9 +186,9 @@ theorem compromise.spec
   [BytesFunctor] [BytesInvariants] [BytesInvariantsProofs]
   [PersistentGlobalState.GlobalStateInv StateT]
   [Comparse.ParseableSerializeable StateT]
-  [TraceTypes.Has Network.ProofEntryFunc] [TraceInvariant.Has Network.Invariant]
-  [TraceTypes.Has (PersistentGlobalState.ProofEntryFunc StateT)] [TraceInvariant.Has (PersistentGlobalState.Invariant StateT)]
-  [TraceTypes.Has (ProtocolEvent.ProofEntryFunc (CompromiseEvent StateT))] [TraceInvariant.Has (ProtocolEvent.Invariant (CompromiseEvent StateT))]
+  [TraceTypes.Has Network.ProofEntryT] [TraceInvariant.Has Network.ProofEntryT]
+  [TraceTypes.Has (PersistentGlobalState.ProofEntryT StateT)] [TraceInvariant.Has (PersistentGlobalState.ProofEntryT StateT)]
+  [TraceTypes.Has (ProofEntryT StateT)] [TraceInvariant.Has (ProofEntryT StateT)]
   [CompromisableStateInv StateT]
   (i: Nat)
   : HoareTriple
@@ -124,5 +205,7 @@ theorem compromise.spec
     have : (label state).isCorrupt tr.erase := by simp_all [label, ProtocolEvent.label_isCorrupt]
     grind [Comparse.isWellFormed, canFlowTrans]
   trivial
+
+end Proof
 
 end DY.Compromise
