DY/Actions/PersistentLocalState.lean
@@ -8,6 +8,8 @@ import DY.Step.Init
 
 namespace DY.PersistentLocalState
 
+section Execution
+
 public
 abbrev Participant := String
 
@@ -16,17 +18,73 @@ structure LocalState (StateT: Type) where
   participant: Participant
   state: StateT
 
+
+@[expose]
 public
-abbrev ExecEntryT (StateT: Type) := PersistentGlobalState.ExecEntryT (LocalState StateT)
+def ExecEntryT.internal (StateT: Type): Fin 1 → Type
+  | 0 => PersistentGlobalState.ExecEntryT (LocalState StateT)
 
 public
-abbrev baseAttackerKnowledge [BytesFunctor] [ExecTraceTypes] (StateT: Type) := PersistentGlobalState.baseAttackerKnowledge (LocalState StateT)
+abbrev ExecEntryT (StateT: Type): Type :=
+  ExecTraceTypes.combine (ExecEntryT.internal StateT)
 
 public
-abbrev ProofEntryT (StateT: Type) := PersistentGlobalState.ProofEntryT (LocalState StateT)
+instance (StateT: Type): ExecTraceTypes.HasStep (PersistentGlobalState.ExecEntryT (LocalState StateT)) (ExecEntryT StateT) :=
+  inferInstanceAs (ExecTraceTypes.HasStep (ExecEntryT.internal StateT 0) (ExecTraceTypes.combine (ExecEntryT.internal StateT)))
 
 public
-abbrev ProofEntryFunc (StateT: Type) := PersistentGlobalState.ProofEntryFunc (LocalState StateT)
+def baseAttackerKnowledge.internal [BytesFunctor] [ExecTraceTypes] (StateT: Type): (id: Fin 1) → SubBaseAttackerKnowledge (ExecEntryT.internal StateT id)
+  | 0 => PersistentGlobalState.baseAttackerKnowledge (LocalState StateT)
+
+public
+def baseAttackerKnowledge [BytesFunctor] [ExecTraceTypes] (StateT: Type): SubBaseAttackerKnowledge (ExecEntryT StateT) :=
+  SubBaseAttackerKnowledge.combine (baseAttackerKnowledge.internal StateT)
+
+public
+def storeLocalState
+  {StateT: Type}
+  [ExecTraceTypes] [ExecTraceTypes.Has (ExecEntryT StateT)]
+  (participant: Participant) (state: StateT)
+  : Traceful Nat
+:= do
+  PersistentGlobalState.storeGlobalState ({ participant, state }: LocalState StateT)
+
+public
+def getLocalState
+  {StateT: Type}
+  [ExecTraceTypes] [ExecTraceTypes.Has (ExecEntryT StateT)]
+  (participant: Participant) (i: Nat)
+  : Traceful StateT
+:= do
+  let st: LocalState StateT ← PersistentGlobalState.getGlobalState i
+  guard (st.participant = participant)
+  return st.state
+
+end Execution
+
+section Proof
+
+@[expose]
+public
+def ProofEntryT.internal (StateT: Type): Fin 1 → Type
+  | 0 => PersistentGlobalState.ProofEntryT (LocalState StateT)
+
+public
+abbrev ProofEntryT (StateT: Type): Type :=
+  TraceTypes.combine (ProofEntryT.internal StateT)
+
+public
+instance (StateT: Type): ∀ id, ErasableProofEntry (ExecEntryT.internal StateT id) (ProofEntryT.internal StateT id)
+  | 0 => by dsimp only [ExecEntryT.internal, ProofEntryT.internal]; infer_instance
+
+public
+instance (StateT: Type): ErasableProofEntry (ExecEntryT StateT) (ProofEntryT StateT) := by
+  dsimp only [ExecEntryT, ProofEntryT]
+  infer_instance
+
+public
+instance (StateT: Type): TraceTypes.HasStep (PersistentGlobalState.ProofEntryT (LocalState StateT)) (ProofEntryT StateT) :=
+  inferInstanceAs (TraceTypes.HasStep (ProofEntryT.internal StateT 0) (TraceTypes.combine (ProofEntryT.internal StateT)))
 
 public
 class LocalStateInv [TraceTypes] (StateT: Type) where
@@ -49,19 +107,38 @@ where
   invariant_later st tr1 tr2 := LocalStateInv.invariant_later st.participant st.state tr1 tr2
 
 public
-abbrev Invariant [TraceTypes] (StateT: Type) [LocalStateInv StateT] := PersistentGlobalState.Invariant (LocalState StateT)
+instance [TraceTypes] (StateT: Type) [LocalStateInv StateT]: ∀ id, ProofEntryInvariant (ProofEntryT.internal StateT id)
+  | 0 => by dsimp only [ProofEntryT.internal]; infer_instance
 
 public
-def baseAttackerKnowledgeTheorem [TraceInvariant] [BytesFunctor] [BytesInvariants] (StateT: Type) [TraceTypes.Has (ProofEntryFunc StateT)] [LocalStateInv StateT] [TraceInvariant.Has (Invariant StateT)] := PersistentGlobalState.baseAttackerKnowledgeTheorem (LocalState StateT)
+instance [TraceTypes] (StateT: Type) [LocalStateInv StateT]: ProofEntryInvariant (ProofEntryT StateT) := by dsimp only [ProofEntryT]; infer_instance
 
 public
-def storeLocalState
-  {StateT: Type}
-  [ExecTraceTypes] [ExecTraceTypes.Has (ExecEntryT StateT)]
-  (participant: Participant) (state: StateT)
-  : Traceful Nat
-:= do
-  PersistentGlobalState.storeGlobalState ({ participant, state }: LocalState StateT)
+instance [TraceTypes] (StateT: Type) [LocalStateInv StateT]: TraceInvariant.HasStep (PersistentGlobalState.ProofEntryT (LocalState StateT)) (ProofEntryT StateT) :=
+  inferInstanceAs (TraceInvariant.HasStep (ProofEntryT.internal StateT 0) (TraceTypes.combine (ProofEntryT.internal StateT)))
+
+public
+instance
+  [TraceInvariant] [BytesFunctor] [BytesInvariants]
+  (StateT: Type)
+  [LocalStateInv StateT]
+  [TraceTypes.Has (ProofEntryT StateT)]
+  [TraceInvariant.Has (ProofEntryT StateT)]
+  : ∀ id, SubBaseAttackerKnowledgeTheorem (ProofEntryT.internal StateT id) (baseAttackerKnowledge.internal StateT id)
+  -- TODO: investigate why infer_instance doesn't work
+  | 0 => by dsimp only [ProofEntryT.internal, baseAttackerKnowledge.internal]; apply PersistentGlobalState.baseAttackerKnowledgeTheorem
+
+public
+instance baseAttackerKnowledgeTheorem
+  [TraceInvariant] [BytesFunctor] [BytesInvariants]
+  (StateT: Type)
+  [LocalStateInv StateT]
+  [TraceTypes.Has (ProofEntryT StateT)]
+  [TraceInvariant.Has (ProofEntryT StateT)]
+  : SubBaseAttackerKnowledgeTheorem (ProofEntryT StateT) (baseAttackerKnowledge StateT)
+:= by
+  dsimp only [ProofEntryT, baseAttackerKnowledge]
+  infer_instance
 
 @[instance]
 public
@@ -69,7 +146,7 @@ theorem storeLocalState.spec
   {StateT: Type}
   [TraceInvariant]
   [LocalStateInv StateT]
-  [TraceTypes.Has (ProofEntryFunc StateT)] [TraceInvariant.Has (Invariant StateT)]
+  [TraceTypes.Has (ProofEntryT StateT)] [TraceInvariant.Has (ProofEntryT StateT)]
   (participant: Participant) (state: StateT)
   : HoareTriple
     (storeLocalState participant state)
@@ -81,24 +158,13 @@ theorem storeLocalState.spec
   step by simp_all [PersistentGlobalState.GlobalStateInv.invariant]
   trivial
 
-public
-def getLocalState
-  {StateT: Type}
-  [ExecTraceTypes] [ExecTraceTypes.Has (ExecEntryT StateT)]
-  (participant: Participant) (i: Nat)
-  : Traceful StateT
-:= do
-  let st: LocalState StateT ← PersistentGlobalState.getGlobalState i
-  guard (st.participant = participant)
-  return st.state
-
 @[instance]
 public
 theorem getLocalState.spec
   {StateT: Type}
   [TraceInvariant]
   [LocalStateInv StateT]
-  [TraceTypes.Has (ProofEntryFunc StateT)] [TraceInvariant.Has (Invariant StateT)]
+  [TraceTypes.Has (ProofEntryT StateT)] [TraceInvariant.Has (ProofEntryT StateT)]
   (participant: Participant) (i: Nat)
   : HoareTriple
     (getLocalState participant i: Traceful StateT)
@@ -115,7 +181,7 @@ theorem getLocalState.spec
 public
 def LocalStateCompromised
   {StateT: Type}
-  [ExecTraceTypes] [ExecTraceTypes.Has (ProtocolEvent.ExecEntryT (Compromise.CompromiseEvent (LocalState StateT)))] -- ugh
+  [ExecTraceTypes] [ExecTraceTypes.Has (Compromise.ExecEntryT (LocalState StateT))] -- ugh
   (participant: Participant) (state: StateT)
   (tr: ExecTrace)
   : Prop
@@ -125,7 +191,7 @@ def LocalStateCompromised
 public
 theorem LocalStateCompromised_le
   {StateT: Type}
-  [ExecTraceTypes] [ExecTraceTypes.Has (ProtocolEvent.ExecEntryT (Compromise.CompromiseEvent (LocalState StateT)))] -- ugh
+  [ExecTraceTypes] [ExecTraceTypes.Has (Compromise.ExecEntryT (LocalState StateT))] -- ugh
   (participant: Participant) (state: StateT)
   (tr1 tr2: ExecTrace)
   : tr1 ≤ tr2 →
@@ -140,7 +206,7 @@ grind_pattern LocalStateCompromised_le => tr1 ≤ tr2, LocalStateCompromised par
 public
 def label
   {StateT: Type}
-  [ExecTraceTypes] [ExecTraceTypes.Has (ProtocolEvent.ExecEntryT (Compromise.CompromiseEvent (LocalState StateT)))] -- ugh
+  [ExecTraceTypes] [ExecTraceTypes.Has (Compromise.ExecEntryT (LocalState StateT))] -- ugh
   (participant: Participant) (state: StateT)
 :=
   Compromise.label ({ participant, state }: LocalState StateT)
@@ -148,7 +214,7 @@ def label
 public
 theorem label_isCorrupt
   {StateT: Type}
-  [ExecTraceTypes] [ExecTraceTypes.Has (ProtocolEvent.ExecEntryT (Compromise.CompromiseEvent (LocalState StateT)))] -- ugh
+  [ExecTraceTypes] [ExecTraceTypes.Has (Compromise.ExecEntryT (LocalState StateT))] -- ugh
   (participant: Participant) (state: StateT)
   (tr: ExecTrace)
   : (label participant state).isCorrupt tr = LocalStateCompromised participant state tr
@@ -164,7 +230,7 @@ class CompromisableStateInv
   [BytesFunctor] [BytesInvariants]
   [Comparse.ParseableSerializeable StateT]
   [LocalStateInv StateT]
-  [ExecTraceTypes.Has (ProtocolEvent.ExecEntryT (Compromise.CompromiseEvent (LocalState StateT)))] -- ugh
+  [ExecTraceTypes.Has (Compromise.ExecEntryT (LocalState StateT))] -- ugh
 where
   invariant_implies_KnowableBy:
     ∀ (participant: Participant) (state: StateT) tr,
@@ -191,7 +257,7 @@ instance
   (StateT: Type)
   [Comparse.ParseableSerializeable StateT]
   [LocalStateInv StateT]
-  [ExecTraceTypes.Has (ProtocolEvent.ExecEntryT (Compromise.CompromiseEvent (LocalState StateT)))] -- ugh
+  [ExecTraceTypes.Has (Compromise.ExecEntryT (LocalState StateT))] -- ugh
   [CompromisableStateInv StateT]
   : Compromise.CompromisableStateInv (LocalState StateT)
 where
@@ -200,5 +266,7 @@ where
     have := CompromisableStateInv.invariant_implies_KnowableBy participant state tr
     simp [PersistentGlobalState.GlobalStateInv.invariant]
     grind
+
+end Proof
 
 end DY.PersistentLocalState
